incomplete ParLang to SrcProg translation

examples/ParLang/ParLangToSrcProg.v
@@ -6,15 +6,19 @@ Print Source.
 (*
 Parallel -> SrcProg
 Cond     -> FlatFormula
-ParTerm  -> NowTerm (missing a lot of math operators...)
- *)
+ParTerm  -> NowTerm
+*)
+Print eval_SrcProg.
 
-Definition Par_Abstracts_SrcProg
-  {ins outs} (par : Parallel ins outs) (sp : SrcProg)
-  : Prop :=
-  forall st1 st2 fst1 fst2,
-    (eval_SrcProg sp fst1) = Some fst2 ->
-    eval_Parallel par st1 = st2.
+(* How to relate fstates and par states?? *)
+(* Definition Par_Abstracts_SrcProg
+ *   {ins outs} (p : Parallel ins outs) (sp : SrcProg)
+ *   : Prop :=
+ *   forall st1 st2 fst1 fst2,
+ *     (eval_SrcProg sp fst1) = Some fst2 ->
+ *     (forall x, In x outs -> fst1 x = st2 x) ->
+ *     eval_Parallel p st1 = st2.
+ *)
 
 Definition Cond_Abstracts_FlatFormula
   {ins} (c : Cond ins) (ff : FlatFormula)
@@ -23,9 +27,47 @@ Definition Cond_Abstracts_FlatFormula
     (progr_cond_holds fst ff) = Some b ->
     eq (eval_Cond c st) b.
 
+Print fstate.
+Print eval_ParTerm.
+
 Definition ParTerm_Abstracts_NowTerm
-           {ins} (pt : ParTerm ins) (nt : NowTerm)
+  {ins} (pt : ParTerm ins) (nt : NowTerm)
   : Prop :=
   forall st fst f,
     eval_NowTerm fst nt = Some f ->
     eval_ParTerm pt st = FloatToR f.
+
+Print NowTerm.
+Require Import ExtLib.Structures.Monad.
+
+Fixpoint Par_To_Now {xs} (pt: ParTerm xs) {struct pt} : option NowTerm :=
+  match pt with
+  | VarPT v => Some (VarNowN v)
+  | NatPT n => Some (NatN n)
+  | RealPT r => None
+  | PlusPT _ _ a b =>
+    bind (Par_To_Now a)
+         (fun a1 =>
+            bind (Par_To_Now b)
+                 (fun b1 => ret (PlusN a1 b1)))
+  | MinusPT _ _ a b =>
+    bind (Par_To_Now a)
+         (fun a1 =>
+            bind (Par_To_Now b)
+                 (fun b1 => ret (MinusN a1 b1)))
+  | MultPT _ _ a b =>
+      bind (Par_To_Now a)
+         (fun a1 =>
+            bind (Par_To_Now b)
+                 (fun b1 => ret (MultN a1 b1)))
+  | _ => None
+  end.
+
+Lemma Par_To_Now_sound :
+  forall xs pt nt,
+  @Par_To_Now xs pt = Some nt ->
+  ParTerm_Abstracts_NowTerm pt nt.
+Proof.
+  induction pt; simpl; try solve [intros; congruence].
+  { intros. inversion H. subst. red. simpl. intros.
+Abort.
